src/Mail2/FindAvailableImpl.v
@@ -3,14 +3,14 @@ Require Import String.
 Require Import CreateAPI.
 
 
-Module FindAvailable <: LayerImpl RestrictedListAPI MaildirAPI.
+Module FindAvailable <: LayerImplFollowsRule RestrictedListAPI MaildirAPI LinkMsgRule.
 
   Fixpoint nextfn (files : list string) (r : string) : string :=
     match files with
     | nil => r
     | fn' :: files' =>
       let r' :=
-        if (lt_dec (String.length r) (String.length fn')) then
+        if (le_dec (String.length r) (String.length fn')) then
           ("a" ++ fn')%string
         else
           r
@@ -18,18 +18,47 @@ Module FindAvailable <: LayerImpl RestrictedListAPI MaildirAPI.
       nextfn files' r'
     end.
 
+  Lemma nextfn_ok' : forall (tid : nat) `(s : FMap.t _ V) r1 r0 n,
+    ( forall fn, FMap.In (tid, fn) s -> In fn (r0 ++ r1) ) ->
+    ( forall fn, In fn r0 -> String.length n > String.length fn ) ->
+    ~ FMap.In (tid, nextfn r1 n) s.
+  Proof.
+    induction r1; simpl; intros.
+    - intro.
+      specialize (H _ H1). rewrite app_nil_r in *.
+      specialize (H0 _ H).
+      omega.
+    - eapply IHr1 with (r0 := r0 ++ (a :: nil)); clear IHr1; intros.
+      + rewrite <- app_assoc; simpl. eauto.
+      + eapply in_app_or in H1; intuition eauto.
+        * specialize (H0 _ H2).
+          destruct (le_dec (length n) (length a)); simpl; omega.
+        * inversion H2; subst. 2: inversion H1.
+          destruct (le_dec (length n) (length fn)); simpl; omega.
+  Qed.
+
+  Lemma nextfn_ok : forall (tid : nat) `(s : FMap.t _ V) r n,
+    ( forall fn, In fn r <-> FMap.In (tid, fn) s ) ->
+    ~ FMap.In (tid, nextfn r n) s.
+  Proof.
+    intros.
+    eapply nextfn_ok' with (r0 := nil); simpl; intros.
+    eapply H; eauto.
+    omega.
+  Qed.
+
   Definition linkmsg_core (data : string) :=
-    files <- Op RestrictedListAPI.ListRestricted;
+    files <- Op RL2API.ListRestricted;
     let newname := nextfn files ""%string in
-    _ <- Op (RestrictedListAPI.LinkMsg newname data);
+    _ <- Op (RL2API.LinkMsg newname data);
     Ret tt.
 
   Definition list_core :=
-    l <- Op (RestrictedListAPI.List);
+    l <- Op (RL2API.List);
     Ret l.
 
   Definition readmsg_core fn :=
-    r <- Op (RestrictedListAPI.ReadMsg fn);
+    r <- Op (RL2API.ReadMsg fn);
     Ret r.
 
   Definition compile_op T (op : MaildirAPI.opT T) : proc _ T :=
@@ -45,25 +74,32 @@ Module FindAvailable <: LayerImpl RestrictedListAPI MaildirAPI.
       inversion H; clear H; subst; repeat sigT_eq
     | H : RestrictedListAPI.step _ _ _ _ _ _ |- _ =>
       inversion H; clear H; subst; repeat sigT_eq
+    | H : RestrictedListAPI.step_allow _ _ _ |- _ =>
+      inversion H; clear H; subst; repeat sigT_eq
+    | H : RL2API.step _ _ _ _ _ _ |- _ =>
+      inversion H; clear H; subst; repeat sigT_eq
     end; intuition idtac.
 
   Hint Extern 1 (MaildirAPI.step _ _ _ _ _ _) => econstructor.
   Hint Extern 1 (RestrictedListAPI.step _ _ _ _ _ _) => econstructor.
+  Hint Extern 1 (RestrictedListAPI.step_allow _ _ _) => econstructor.
+  Hint Extern 1 (RL2API.step _ _ _ _ _ _) => econstructor.
 
   Lemma listrestricted_right_mover :
     right_mover
       RestrictedListAPI.step
-      (RestrictedListAPI.ListRestricted).
+      (RL2API.ListRestricted).
   Proof.
     unfold right_mover; intros.
-    repeat step_inv; eauto.
+    repeat step_inv; eauto 10.
     eexists; split.
     econstructor; eauto.
-    econstructor; intros.
+    econstructor; intros; eauto.
+    econstructor; intros; eauto.
     split; intros.
-    - eapply H1 in H0.
+    - eapply H3 in H0.
       eapply FMap.in_add; eauto.
-    - eapply H1.
+    - eapply H3.
       eapply FMap.in_add_ne; eauto.
       congruence.
   Qed.
@@ -182,10 +218,173 @@ Module FindAvailable <: LayerImpl RestrictedListAPI MaildirAPI.
     eauto.
   Qed.
 
+  Lemma list_follows_protocol : forall tid s,
+    follows_protocol_proc RL2API.step RestrictedListAPI.step_allow LinkMsgRule.loopInv tid s list_core.
+  Proof.
+    intros.
+    constructor; intros.
+      constructor; intros. eauto.
+    constructor; intros.
+  Qed.
+
+  Lemma readmsg_follows_protocol : forall tid s fn,
+    follows_protocol_proc RL2API.step RestrictedListAPI.step_allow LinkMsgRule.loopInv tid s (readmsg_core fn).
+  Proof.
+    intros.
+    constructor; intros.
+      constructor; intros. eauto.
+    constructor; intros.
+  Qed.
+
+  Lemma linkmsg_follows_protocol : forall tid s data,
+    follows_protocol_proc RL2API.step RestrictedListAPI.step_allow LinkMsgRule.loopInv tid s (linkmsg_core data).
+  Proof.
+    intros.
+    constructor; intros.
+      constructor; intros. eauto.
+
+    constructor; intros.
+      constructor; intros.
+
+    {
+      eapply exec_any_op in H; repeat deex.
+      destruct H0.
+      repeat step_inv.
+
+      econstructor.
+      eapply nextfn_ok; eauto.
+    }
+
+    constructor; intros.
+  Qed.
+
+  Hint Resolve linkmsg_follows_protocol.
+  Hint Resolve readmsg_follows_protocol.
+  Hint Resolve list_follows_protocol.
+
+  Theorem compile_ts_follows_protocol :
+    forall ts,
+      no_atomics_ts ts ->
+      LinkMsgRule.follows_protocol (compile_ts ts).
+  Proof.
+    unfold compile_ts.
+    unfold LinkMsgRule.follows_protocol.
+    unfold follows_protocol_s.
+    intros.
+
+    edestruct proc_match_pick with (tid := tid).
+      eapply Compile.compile_ts_ok with (compile_op := compile_op); eauto.
+    unfold RL2API.opT, RestrictedListAPI.opT in *.
+      intuition congruence.
+    unfold RL2API.opT, RestrictedListAPI.opT in *.
+      repeat deex.
+    match goal with
+    | H1 : _ [[ tid ]] = Proc _,
+      H2 : _ [[ tid ]] = Proc _ |- _ =>
+      rewrite H1 in H2; clear H1; inversion H2; clear H2;
+        subst; repeat sigT_eq
+    end.
+
+    clear dependent ts.
+    generalize dependent s.
+
+    match goal with
+    | H : Compile.compile_ok _ _ _ |- _ =>
+      induction H; intros; eauto
+    end.
+
+    destruct op; simpl; eauto.
+
+    unfold LinkMsgRule.loopInv.
+    econstructor; eauto.
+  Qed.
+
 End FindAvailable.
 
 
-Module RLImpl <: LayerImpl RawDirAPI RestrictedListAPI.
+Module RLImpl <: LayerImplRequiresRule RL2API RestrictedListAPI LinkMsgRule.
+
+  Import LinkMsgRule.
+
+  Definition absR (s1 : RL2API.State) (s2 : RestrictedListAPI.State) :=
+    s1 = s2.
+
+  Ltac step_inv :=
+    match goal with
+    | H : RL2API.step _ _ _ _ _ _ |- _ =>
+      inversion H; clear H; subst; repeat sigT_eq
+    | H : RestrictedListAPI.step_allow _ _ _ |- _ =>
+      inversion H; clear H; subst; repeat sigT_eq
+    | H : RestrictedListAPI.step _ _ _ _ _ _ |- _ =>
+      destruct H; intuition idtac
+    end.
+
+  Theorem allowed_stable :
+    forall `(op : RestrictedListAPI.opT T) `(op' : RestrictedListAPI.opT T') tid tid' s s' r evs,
+      tid <> tid' ->
+      RestrictedListAPI.step_allow op tid s ->
+      RestrictedListAPI.step op' tid' s r s' evs ->
+      RestrictedListAPI.step_allow op tid s'.
+  Proof.
+    intros.
+    destruct op; destruct op'; repeat step_inv; subst; eauto.
+    constructor.
+    contradict H4.
+    eapply FMap.in_add_ne; eauto.
+    congruence.
+  Qed.
+
+  Definition compile_ts (ts : @threads_state RestrictedListAPI.opT) := ts.
+
+  Theorem compile_ts_no_atomics :
+    forall ts,
+      no_atomics_ts ts ->
+      no_atomics_ts (compile_ts ts).
+  Proof.
+    unfold compile_ts; eauto.
+  Qed.
+
+  Theorem absInitP :
+    forall s1 s2,
+      RL2API.initP s1 ->
+      absR s1 s2 ->
+      RestrictedListAPI.initP s2.
+  Proof.
+    eauto.
+  Qed.
+
+  Theorem compile_traces_match :
+    forall ts,
+      follows_protocol ts ->
+      no_atomics_ts ts ->
+      traces_match_abs absR RL2API.initP RL2API.step RestrictedListAPI.step (compile_ts ts) ts.
+  Proof.
+    unfold compile_ts, follows_protocol, absR.
+    unfold traces_match_abs; intros; subst.
+    clear H1.
+    specialize (H sm).
+    destruct H2.
+    induction H1; eauto.
+    specialize (H tid _ p) as Htid.
+    intuition idtac; repeat deex.
+
+    edestruct IHexec.
+      eapply follows_protocol_s_exec_tid_upd; eauto.
+      intros; eapply allowed_stable; eauto.
+      destruct result; eauto.
+
+    eexists; intuition idtac.
+    eapply ExecPrefixOne.
+      eauto.
+      eapply follows_protocol_preserves_exec_tid'; eauto.
+      eauto.
+    eauto.
+  Qed.
+
+End RLImpl.
+
+
+Module RL2Impl <: LayerImpl RawDirAPI RL2API.
 
   Definition same_tid (tid : nat) (fn : nat * string) : bool :=
     if tid == fst fn then
@@ -194,8 +393,8 @@ Module RLImpl <: LayerImpl RawDirAPI RestrictedListAPI.
       false.
 
   Definition linkmsg_core newname data :=
-    _ <- Op (RawDirAPI.LinkMsg newname data);
-    Ret tt.
+    v <- Op (RawDirAPI.LinkMsg newname data);
+    Ret v.
 
   Definition list_core :=
     l <- Op (RawDirAPI.List);
@@ -210,24 +409,24 @@ Module RLImpl <: LayerImpl RawDirAPI RestrictedListAPI.
     r <- Op (RawDirAPI.ReadMsg fn);
     Ret r.
 
-  Definition compile_op T (op : RestrictedListAPI.opT T) : proc _ T :=
+  Definition compile_op T (op : RL2API.opT T) : proc _ T :=
     match op with
-    | RestrictedListAPI.LinkMsg fn m => linkmsg_core fn m
-    | RestrictedListAPI.List => list_core
-    | RestrictedListAPI.ListRestricted => list_restricted_core
-    | RestrictedListAPI.ReadMsg fn => readmsg_core fn
+    | RL2API.LinkMsg fn m => linkmsg_core fn m
+    | RL2API.List => list_core
+    | RL2API.ListRestricted => list_restricted_core
+    | RL2API.ReadMsg fn => readmsg_core fn
     end.
 
   Ltac step_inv :=
     match goal with
     | H : RawDirAPI.step _ _ _ _ _ _ |- _ =>
       inversion H; clear H; subst; repeat sigT_eq
-    | H : RestrictedListAPI.step _ _ _ _ _ _ |- _ =>
+    | H : RL2API.step _ _ _ _ _ _ |- _ =>
       inversion H; clear H; subst; repeat sigT_eq
     end; intuition idtac.
 
   Hint Extern 1 (RawDirAPI.step _ _ _ _ _ _) => econstructor.
-  Hint Extern 1 (RestrictedListAPI.step _ _ _ _ _ _) => econstructor.
+  Hint Extern 1 (RL2API.step _ _ _ _ _ _) => econstructor.
 
   Lemma gettid_right_mover :
     right_mover
@@ -242,8 +441,8 @@ Module RLImpl <: LayerImpl RawDirAPI RestrictedListAPI.
 
   Theorem linkmsg_atomic : forall `(rx : _ -> proc _ T) fn m,
     trace_incl RawDirAPI.step
-      (Bind (compile_op (RestrictedListAPI.LinkMsg fn m)) rx)
-      (Bind (atomize compile_op (RestrictedListAPI.LinkMsg fn m)) rx).
+      (Bind (compile_op (RL2API.LinkMsg fn m)) rx)
+      (Bind (atomize compile_op (RL2API.LinkMsg fn m)) rx).
   Proof.
     intros.
     eapply trace_incl_atomize_ysa.
@@ -254,8 +453,8 @@ Module RLImpl <: LayerImpl RawDirAPI RestrictedListAPI.
 
   Theorem list_atomic : forall `(rx : _ -> proc _ T),
     trace_incl RawDirAPI.step
-      (Bind (compile_op (RestrictedListAPI.List)) rx)
-      (Bind (atomize compile_op (RestrictedListAPI.List)) rx).
+      (Bind (compile_op (RL2API.List)) rx)
+      (Bind (atomize compile_op (RL2API.List)) rx).
   Proof.
     intros.
     eapply trace_incl_atomize_ysa.
@@ -266,8 +465,8 @@ Module RLImpl <: LayerImpl RawDirAPI RestrictedListAPI.
 
   Theorem list_restricted_atomic : forall `(rx : _ -> proc _ T),
     trace_incl RawDirAPI.step
-      (Bind (compile_op (RestrictedListAPI.ListRestricted)) rx)
-      (Bind (atomize compile_op (RestrictedListAPI.ListRestricted)) rx).
+      (Bind (compile_op (RL2API.ListRestricted)) rx)
+      (Bind (atomize compile_op (RL2API.ListRestricted)) rx).
   Proof.
     intros.
     eapply trace_incl_atomize_ysa.
@@ -278,8 +477,8 @@ Module RLImpl <: LayerImpl RawDirAPI RestrictedListAPI.
 
   Theorem readmsg_atomic : forall `(rx : _ -> proc _ T) fn,
     trace_incl RawDirAPI.step
-      (Bind (compile_op (RestrictedListAPI.ReadMsg fn)) rx)
-      (Bind (atomize compile_op (RestrictedListAPI.ReadMsg fn)) rx).
+      (Bind (compile_op (RL2API.ReadMsg fn)) rx)
+      (Bind (atomize compile_op (RL2API.ReadMsg fn)) rx).
   Proof.
     intros.
     eapply trace_incl_atomize_ysa.
@@ -289,14 +488,13 @@ Module RLImpl <: LayerImpl RawDirAPI RestrictedListAPI.
   Qed.
 
   Theorem my_compile_correct :
-    compile_correct compile_op RawDirAPI.step RestrictedListAPI.step.
+    compile_correct compile_op RawDirAPI.step RL2API.step.
   Proof.
     unfold compile_correct; intros.
     destruct op.
 
     + repeat atomic_exec_inv.
       repeat step_inv; eauto.
-      admit.
     + repeat atomic_exec_inv.
       repeat step_inv; eauto.
     + repeat atomic_exec_inv.
@@ -315,7 +513,7 @@ Module RLImpl <: LayerImpl RawDirAPI RestrictedListAPI.
         destruct (v1 == v1); congruence.
     + repeat atomic_exec_inv.
       repeat step_inv; eauto.
-  Admitted.
+  Qed.
 
   Theorem my_atomize_correct :
     atomize_correct compile_op RawDirAPI.step.
@@ -342,13 +540,13 @@ Module RLImpl <: LayerImpl RawDirAPI RestrictedListAPI.
   Theorem all_traces_match :
     forall ts1 ts2,
       proc_match (Compile.compile_ok compile_op) ts1 ts2 ->
-      traces_match_ts RawDirAPI.step RestrictedListAPI.step ts1 ts2.
+      traces_match_ts RawDirAPI.step RL2API.step ts1 ts2.
   Proof.
     intros.
     eapply Compile.compile_traces_match_ts; eauto.
   Qed.
 
-  Definition absR (s1 : RawDirAPI.State) (s2 : RestrictedListAPI.State) :=
+  Definition absR (s1 : RawDirAPI.State) (s2 : RL2API.State) :=
     s1 = s2.
 
   Definition compile_ts := Compile.compile_ts compile_op.
@@ -365,7 +563,7 @@ Module RLImpl <: LayerImpl RawDirAPI RestrictedListAPI.
   Theorem compile_traces_match :
     forall ts2,
       no_atomics_ts ts2 ->
-      traces_match_abs absR RawDirAPI.initP RawDirAPI.step RestrictedListAPI.step (compile_ts ts2) ts2.
+      traces_match_abs absR RawDirAPI.initP RawDirAPI.step RL2API.step (compile_ts ts2) ts2.
   Proof.
     unfold traces_match_abs; intros.
     rewrite H2 in *; clear H2.
@@ -382,4 +580,4 @@ Module RLImpl <: LayerImpl RawDirAPI RestrictedListAPI.
     eauto.
   Qed.
 
-End RLImpl.
+End RL2Impl.
